theories/Core/HoareFacts.v
@@ -180,3 +180,64 @@ Proof.
 Qed.
 
 #[global] Hint Resolve to_hoare_contractprod : freespec.
+
+Lemma contract_equ_pre `(c1 : contract i Ω1) `(c2 : contract i Ω2)
+   `(equ : contract_equ c1 c2) (ω1 : Ω1)
+   `(p : impure i a)
+  : pre (to_hoare c1 p) ω1 <-> pre (to_hoare c2 p) (contract_iso_lr equ ω1).
+
+Proof.
+  induction equ.
+  revert ω1.
+  induction p; intros ω1.
+  + now split.
+  + cbn.
+    rewrite (caller_equ ω1 β e).
+    setoid_rewrite (callee_equ ω1 β e).
+    split.
+    ++ intros [ocaller onext].
+       split; auto.
+       intros x ω1' [ocallee owitness].
+       rewrite owitness.
+       rewrite <- witness_equ.
+       rewrite <- H; eauto.
+    ++ intros [ocaller onext].
+       split; auto.
+       intros x ω1' [ocallee owitness].
+       rewrite H; eauto.
+       rewrite owitness.
+       cbn.
+       rewrite witness_equ.
+       eauto.
+Qed.
+
+#[global] Hint Resolve contract_equ_pre : freespec.
+
+Lemma contract_equ_post `(c1 : contract i Ω1) `(c2 : contract i Ω2)
+   `(equ : contract_equ c1 c2) (ω1 ω1' : Ω1)
+   `(p : impure i a) (x : a)
+    (post1 : post (to_hoare c1 p) ω1 x ω1')
+  : post (to_hoare c2 p) (contract_iso_lr equ ω1) x (contract_iso_lr equ  ω1').
+
+Proof.
+  induction equ.
+  cbn in *.
+  revert x ω1 ω1' post1.
+  induction p; intros y ω1 ω1' post1.
+  + destruct post1 as [xequ ω1equ].
+    cbn.
+    now subst.
+  + cbn in post1.
+    destruct post1 as [x [ω1'' [[ocallee owitness] post1]]].
+    eapply H in post1.
+    exists x.
+    exists (f ω1'').
+    split; auto.
+    cbn.
+    repeat split.
+    ++ eapply callee_equ; eauto.
+    ++ rewrite owitness.
+       apply witness_equ.
+Qed.
+
+#[global] Hint Resolve contract_equ_post : freespec.
